src/Model.QUIC.fst
@@ -1,0 +1,249 @@
+module Model.QUIC
+
+module HS = FStar.HyperStack
+module I = Model.Indexing
+module U32 = FStar.UInt32
+module U64 = FStar.UInt64
+module U128 = FStar.UInt128
+module M = LowStar.Modifies
+
+friend QUIC.TotSpec
+
+module Spec = QUIC.Spec
+module TSpec = QUIC.TotSpec
+module QH = QUIC.Spec.Header
+module AE = Model.AEAD
+module SAE = Spec.Agile.AEAD
+module PNE = Model.PNE
+module SPNE = Spec.Agile.Cipher
+module BF = LowParse.BitFields
+module U62 = QUIC.UInt62
+module Secret = QUIC.Secret.Int
+module B = LowStar.Buffer
+
+open FStar.HyperStack.ST
+open FStar.UInt32
+open Mem
+
+type _ctr (offset:pn) = p:pn{p >= offset}
+
+let pne_plain (j:PNE.id) (l:pnl) : eqtype = Spec.lbytes l & PNE.length_bits l
+let as_bytes (j:PNE.id) (l:pnl) (x:pne_plain j l) : GTot (Helpers.lbytes l & PNE.length_bits l) = let (n,b) = x in (Helpers.hide n, b)
+let repr (j:PNE.unsafe_id) (l:pnl) (x:pne_plain j l) : b:(Helpers.lbytes l & PNE.length_bits l){b == as_bytes j l x} =
+  let (n,b)=x in (Helpers.hide n, b)
+let mk (j:PNE.id) (l:pnl) (n:Helpers.lbytes l) (b:PNE.length_bits l) : p:pne_plain j l{as_bytes j l p == (n,b)} = Helpers.reveal n,b
+
+let pnenc (j:PNE.id) (l:pnl) (p:pne_plain j l) (c:PNE.pne_cipherpad)
+  : (l':pnl & pne_plain j l') =
+  let npn, bits = p in
+  let pnm, bm = c in
+  let npn' = QUIC.Spec.Lemmas.xor_inplace npn (Seq.slice (Helpers.reveal pnm) 0 l) in
+  let bits' = BF.set_bitfield bits 0 5 (BF.get_bitfield (bits `FStar.UInt.logxor` bm) 0 5) in
+  let ln = BF.get_bitfield bits' 0 2 + 1 in
+  (| ln, (npn', bits') |)
+  
+  admit()
+
+(*
+    let protected_bits = if MShort? h then 5 else 4 in
+    let f' = BF.set_bitfield (U8.v f) 0 protected_bits (BF.get_bitfield (U8.v f `FStar.UInt.logxor` U8.v (Seq.index mask 0)) 0 protected_bits) in
+
+    let r = Seq.cons (U8.uint_to_t f') (Seq.slice r 1 (Seq.length r)) in
+
+  admit()
+*)
+
+let lemma_xor (j:PNE.id) (l:pnl) (p:(Spec.lbytes l & PNE.length_bits l)) (c:PNE.pne_cipherpad)
+  : Lemma (requires True)
+  (ensures (let (| l', b' |) = pnenc j l p c in
+    let _, bits = as_bytes j l' b' in
+    let l:pnl = LowParse.BitFields.get_bitfield bits 0 2 + 1 in
+    l == (l' <: pnl)))
+  = admit()
+
+let pne_pkg : PNE.pne_plain_pkg =
+ PNE.PNEPlainPkg pne_plain as_bytes repr mk pnenc lemma_xor
+
+noeq type stream_writer' (i:id) = 
+| Writer:
+  info: info ->
+  offset: pn ->
+  siv: Spec.lbytes 12 ->
+  ae: AE.aead_writer (dfst i){(AEAD.wgetinfo ae).AEAD.min_len == 3} ->
+  pne_info: PNE.info (dsnd i){
+    pne_info.PNE.calg == Spec.Agile.AEAD.cipher_alg_of_supported_alg (AEAD.wgetinfo ae).AEAD.alg /\
+    pne_info.PNE.halg == (AEAD.wgetinfo ae).AEAD.halg} ->
+  pne: PNE.pne_state pne_info ->
+  ctr: reference (_ctr offset) ->
+  stream_writer' i
+
+let stream_writer = stream_writer'
+
+type _last (offset:pn) = p:nat{p >= offset /\ p < max_ctr}
+
+noeq type stream_reader' (#i:id) (w:stream_writer i) = 
+| Reader:
+  aer: AE.aead_reader (w.ae) ->
+  last: reference (_last w.offset) ->
+  stream_reader' w
+
+let stream_reader = stream_reader'
+
+let writer_info #k w = w.info
+let reader_info #k #w r = w.info
+
+let writer_ae_info #k w = AEAD.wgetinfo w.ae
+let reader_ae_info #k #w r = AEAD.rgetinfo r.aer
+let writer_pne_info #k w = w.pne_info
+let reader_pne_info #k #w r = w.pne_info
+
+let writer_aead_state #k w = w.ae
+let reader_aead_state #k #w r = r.aer
+
+let writer_pne_state #k w = w.pne
+let reader_pne_state #k #w r = w.pne
+
+let invariant #k w h =
+  AEAD.winvariant w.ae h /\
+  PNE.invariant w.pne h /\
+  h `HS.contains` w.ctr /\
+  AEAD.wfootprint w.ae `B.loc_disjoint` (B.loc_mreference w.ctr) /\
+  PNE.footprint w.pne `B.loc_disjoint` (B.loc_mreference w.ctr) /\
+  PNE.footprint w.pne `B.loc_disjoint` AEAD.wfootprint w.ae
+
+let rinvariant #k #w r h = invariant w h /\
+  h `HS.contains` r.last /\
+  AEAD.wfootprint w.ae `B.loc_disjoint` (B.loc_mreference w.ctr)
+
+let writer_offset #k w = w.offset
+let reader_offset #k #w r = w.offset
+
+let wctrT #k w h = HS.sel h w.ctr
+let wctr #k w = !w.ctr
+
+let writer_static_iv #k w = w.siv
+let reader_static_iv #k #w r = w.siv
+
+let expected_pnT #k #w r h = HS.sel h r.last
+let expected_pn #k #w r = !r.last
+
+let footprint #k w = (AEAD.wfootprint w.ae)
+  `B.loc_union` (PNE.footprint w.pne)
+  `B.loc_union` B.loc_mreference w.ctr
+
+let rfootprint #k #w r = footprint w `B.loc_union` B.loc_mreference r.last
+
+let frame_invariant #k w h0 l h1 =
+  AEAD.wframe_invariant l w.ae h0 h1;
+  PNE.frame_invariant w.pne l h0 h1
+
+let rframe_invariant #k #w r h0 l h1 =
+  AEAD.wframe_invariant l w.ae h0 h1;
+  PNE.frame_invariant w.pne l h0 h1
+
+let wframe_log #k w t h0 l h1 =
+  AEAD.frame_log l w.ae h0 h1
+  
+let rframe_log #k #w r t h0 l h1 =
+  AEAD.frame_log l w.ae h0 h1
+
+let wframe_pnlog #k w t h0 l h1 =
+  PNE.frame_table w.pne l h0 h1
+
+let rframe_pnlog #k #w r t h0 l h1 =
+  PNE.frame_table w.pne l h0 h1
+
+let create k u u1 u2 init =
+  let open Model.Helpers in
+  let alg = u1.AEAD.alg in
+  let siv = random 12 in
+  let h0 = get() in
+  let ae = AEAD.gen (dfst k) u1 in
+  let h1 = get () in  
+  let pne = PNE.create (dsnd k) u2 in
+  let h2 = get () in
+  let ctr = ralloc u.region init in
+  let h3 = get () in 
+  AEAD.wframe_invariant M.loc_none ae h1 h3;
+  PNE.frame_invariant pne M.loc_none h2 h3;
+  if safe k then
+   begin
+    AEAD.frame_log M.loc_none ae h1 h3;
+    PNE.frame_table pne M.loc_none h2 h3
+   end;
+  let r = Writer u init (reveal siv) ae u2 pne ctr in
+  r
+
+let coerce k u u1 u2 init ts =
+  let open Model.Helpers in
+  let alg = u1.AEAD.alg in
+  let siv : Model.Helpers.lbytes 12 = Spec.derive_secret u1.AEAD.halg ts Spec.label_iv 12 in
+  let h0 = get() in
+  let u1 : AEAD.info (dfst k) = u1 in
+  let ae = AEAD.quic_coerce u1 ts in
+  let h1 = get () in
+  let pne = PNE.quic_coerce (dsnd k) u2 ts in
+  let h2 = get () in
+  let ctr = ralloc u.region init in
+  let h3 = get () in 
+  AEAD.wframe_invariant M.loc_none ae h1 h3;
+  PNE.frame_invariant pne M.loc_none h2 h3;
+  let r = Writer u init (reveal siv) ae u2 pne ctr in
+  r
+
+let createReader rgn #k w =
+  let h0 = get () in
+  let last = ralloc rgn (writer_offset w) in
+  let h1 = get () in
+  frame_invariant w h0 M.loc_none h1;
+  let aer = AEAD.gen_reader w.ae in
+  Reader aer last
+
+#push-options "--z3rlimit 30"
+let encrypt #k w h #l p =
+  let open Model.Helpers in
+  let alg = (writer_ae_info w).AEAD.alg in
+  if safe k then
+    let h0 = get () in
+    let ln = Lib.RawIntTypes.uint_to_nat (TSpec.pn_length h) - 1 in
+    let iv = TSpec.iv_for_encrypt_decrypt alg (hide w.siv) h in
+    let iv = Helpers.reveal #12 iv in
+    let aad = Helpers.hide (TSpec.format_header h) in
+    let pno = TSpec.pn_offset h in
+    assume(AEAD.fresh_nonce w.ae iv h0);
+    let c1 = AEAD.encrypt (dfst k) w.ae iv aad l p in
+    let h1 = get () in
+    PNE.frame_invariant w.pne (AEAD.wfootprint w.ae) h0 h1;
+    let sample = (Seq.slice c1 (3-ln) (19-ln)) in
+//    let npn = mk (dsnd k) (ln+1) (Helpers.reveal #(ln+1) (Seq.slice aad pno (pno+ln+1))) ln in
+    admit()
+//    PNE.encrypt w.pne
+  else admit()
+
+(*
+    let k1, k2 = writer_leak w in
+    let plain : Spec.pbytes' (Spec.is_retry h) = (writer_ae_info w).AEAD.plain_pkg.AEAD.repr (dfst k) l p in
+    let r = TSpec.encrypt alg
+    (hide k1) (hide w.siv) (hide k2) h plain in
+    let h0 = get () in
+    w.ctr := !w.ctr + 1;
+    let h1 = get () in
+    AEAD.wframe_invariant (M.loc_mreference w.ctr) w.ae h0 h1;
+    PNE.frame_invariant w.pne (M.loc_mreference w.ctr) h0 h1;
+    r
+#pop-options
+*)
+let decrypt #k #w r cid_len packet =
+  if safe k then
+    admit()
+  else
+    let open Model.Helpers in
+    let k1, k2 = reader_leak r in
+    let expected = expected_pn r in
+    let ea = (writer_ae_info w).AE.alg in
+    match QUIC.TotSpec.decrypt ea (hide k1)
+      (hide (reader_static_iv r)) (hide k2)
+      expected cid_len packet with
+    | Spec.Failure -> M_Failure
+    | _ -> admit()
+ 
